Mess around some more with proof for day 8.

day8.v
@@ -2,6 +2,9 @@ Require Import Coq.ZArith.Int.
 Require Import Coq.Lists.ListSet.
 Require Import Coq.Vectors.VectorDef.
 Require Import Coq.Vectors.Fin.
+Require Import Coq.Program.Equality.
+Require Import Coq.Logic.Eqdep_dec.
+Require Import Coq.Arith.Peano_dec.
 
 Module DayEight (Import M:Int).
   (* We need to coerce natural numbers into integers to add them. *)
@@ -42,27 +45,29 @@ Module DayEight (Import M:Int).
      Not all inputs are valid, so this may fail. *)
   Definition valid_jump_t {n} (pc : fin n) (off : t) : option (fin (S n)) := @clamp (S n) (jump_t pc off).
 
-  Definition weaken_one {n} (f : fin n) : fin (S n).
-  Proof.
-    apply (@cast (n + 1)).
-    + apply L. apply f.
-    + rewrite <- plus_n_Sm. rewrite <- plus_n_O. reflexivity.
-  Defined.
+  Fixpoint weaken_one {n} (f : fin n) : fin (S n) :=
+    match f with
+    | F1 => F1
+    | FS f' => FS (weaken_one f')
+    end.
 
+  (* One modification: we really want to use 'allowed' addresses,
+     a set that shrinks as the program continues, rather than 'visited'
+     addresses, a set that increases as the program continues. *)
   Inductive step_noswap {n} : input n -> state n -> state n -> Prop :=
-    | step_noswap_acc : forall inp pc' v acc t,
+    | step_noswap_add : forall inp pc' v acc t,
         nth inp pc' = (add, t) ->
-        ~ set_mem Fin.eq_dec pc' v = true ->
-        step_noswap inp (weaken_one pc', v, acc) (FS pc', set_add Fin.eq_dec pc' v, M.add acc t)
+        set_mem Fin.eq_dec pc' v = true ->
+        step_noswap inp (weaken_one pc', v, acc) (FS pc', set_remove Fin.eq_dec pc' v, M.add acc t)
     | step_noswap_nop : forall inp pc' v acc t,
         nth inp pc' = (nop, t) ->
-        ~ set_mem Fin.eq_dec pc' v = true ->
-        step_noswap inp (weaken_one pc', v, acc) (FS pc', set_add Fin.eq_dec pc' v, acc)
+        set_mem Fin.eq_dec pc' v = true ->
+        step_noswap inp (weaken_one pc', v, acc) (FS pc', set_remove Fin.eq_dec pc' v, acc)
     | step_noswap_jmp : forall inp pc' pc'' v acc t,
         nth inp pc' = (jmp, t) ->
-        ~ set_mem Fin.eq_dec pc' v = true ->
+        set_mem Fin.eq_dec pc' v = true ->
         valid_jump_t pc' t = Some pc'' ->
-        step_noswap inp (weaken_one pc', v, acc) (pc'', set_add Fin.eq_dec pc' v, acc).
+        step_noswap inp (weaken_one pc', v, acc) (pc'', set_remove Fin.eq_dec pc' v, acc).
 
   Fixpoint nat_to_fin (n : nat) : fin (S n) :=
     match n with
@@ -74,7 +79,7 @@ Module DayEight (Import M:Int).
     | run_noswap_ok : forall inp v acc,
         run_noswap inp (nat_to_fin n, v, acc) (nat_to_fin n, v, acc)
     | run_noswap_fail : forall inp pc' v acc,
-        set_mem Fin.eq_dec pc' v = true ->
+        set_mem Fin.eq_dec pc' v = false ->
         run_noswap inp (weaken_one pc', v, acc) (weaken_one pc', v, acc)
     | run_noswap_trans : forall inp st st' st'',
         step_noswap inp st st' -> run_noswap inp st' st'' -> run_noswap inp st st''.
@@ -90,9 +95,323 @@ Module DayEight (Import M:Int).
   Definition valid_input {n} (inp : input n) : Prop := forall (pc : fin n),
     valid_inst (nth inp pc) pc.
 
+  Lemma fin_big_or_small : forall {n} (f : fin (S n)),
+    (f = nat_to_fin n) \/ (exists (f' : fin n), f = weaken_one f').
+  Proof.
+    (* Hey, looks like the creator of Fin provided
+       us with nice inductive principles. Using Coq's
+       default `induction` breaks here.
+
+       Merci, Pierre! *)
+    apply Fin.rectS.
+    - intros n. destruct n.
+      + left. reflexivity.
+      + right. exists F1. auto.
+    - intros n p IH.
+      destruct IH.
+      + left. rewrite H. reflexivity.
+      + right. destruct H as [f' Heq]. 
+        exists (FS f'). simpl. rewrite Heq.
+        reflexivity.
+  Qed.
+
+  Lemma set_add_idempotent : forall {A:Type}
+    (Aeq_dec : forall x y : A, { x = y } + { x <> y })
+    (a : A) (s : set A), set_mem Aeq_dec a s = true -> set_add Aeq_dec a s = s.
+  Proof.
+    intros A Aeq_dec a s Hin.
+    induction s.
+    - inversion Hin.
+    - simpl. simpl in Hin.
+      destruct (Aeq_dec a a0).
+      + reflexivity.
+      + simpl. rewrite IHs; auto.
+  Qed.
+  
+  Theorem set_add_append : forall {A:Type}
+    (Aeq_dec : forall x y : A, {x = y } + { x <> y })
+    (a : A) (s : set A), set_mem Aeq_dec a s = false ->
+    set_add Aeq_dec a s = List.app s (List.cons a List.nil).
+  Proof.
+    induction s.
+    - reflexivity.
+    - intros Hnm. simpl in Hnm.
+      destruct (Aeq_dec a a0) eqn:Heq_dec.
+      + inversion Hnm.
+      + simpl. rewrite Heq_dec. rewrite IHs.
+        reflexivity. assumption.
+  Qed.
+
+  Lemma list_append_or_nil : forall {A:Type} (l : list A),
+    l = List.nil \/ exists l' a, l = List.app l' (List.cons a List.nil).
+  Proof.
+    induction l.
+    - left. reflexivity.
+    - right. destruct IHl.
+      + exists List.nil. exists a.
+        rewrite H. reflexivity.
+      + destruct H as [l' [a' H]].
+        exists (List.cons a l'). exists a'.
+        rewrite H. reflexivity.
+  Qed.
+
+  Theorem list_append_induction : forall {A:Type}
+    (P : list A -> Prop),
+    P List.nil -> (forall (a : A) (l : list A), P l -> P (List.app l (List.cons a (List.nil)))) ->
+    forall l, P l.
+  Proof. Admitted.
+
+
+  Theorem set_induction : forall {A:Type}
+    (Aeq_dec : forall x y : A, { x = y } + {x <> y })
+    (P : set A -> Prop),
+    P (@empty_set A) -> (forall (a : A) (s' : set A), P s' -> P (set_add Aeq_dec a s')) ->
+    forall (s : set A), P s.
+  Proof. Admitted.
+
+  Lemma weaken_one_inj : forall n (f1 f2 : fin n),
+    (weaken_one f1 = weaken_one f2 -> f1 = f2).
+  Proof. 
+    remember (fun {n} (a b : fin n) => weaken_one a = weaken_one b -> a = b) as P.
+    (* Base case for rect2 *)
+    assert (forall n, @P (S n) F1 F1).
+    {rewrite HeqP. intros n Heq. reflexivity. }
+    (* 'Impossible' cases for rect2. *)
+    assert (forall {n} (f : fin n), P (S n) F1 (FS f)).
+    {rewrite HeqP. intros n f Heq. simpl in Heq. inversion Heq. }
+    assert (forall {n} (f : fin n), P (S n) (FS f) F1).
+    {rewrite HeqP. intros n f Heq. simpl in Heq. inversion Heq. }
+    (* Recursive case for rect2. *)
+    assert (forall {n} (f g : fin n), P n f g -> P (S n) (FS f) (FS g)).
+    {rewrite HeqP. intros n f g IH Heq.
+      simpl in Heq. injection Heq as Heq'.
+      apply inj_pair2_eq_dec in Heq'.
+      - rewrite IH. reflexivity. assumption.
+      - apply eq_nat_dec. }
+
+    (* Actually apply recursion. *)
+    (* This can't be _the_ way to do this. *)
+    intros n.
+    specialize (@Fin.rect2 P H H0 H1 H2 n) as Hind.
+    rewrite HeqP in Hind. apply Hind.
+  Qed.
+
+  Lemma weaken_neq_to_fin : forall {n} (f : fin (S n)),
+    nat_to_fin (S n) <> weaken_one f.
+  Proof.
+    apply Fin.rectS; intros n Heq.
+    - inversion Heq.
+    - intros IH. simpl. intros Heq'.
+      injection Heq' as Hinj. apply inj_pair2_eq_dec in Hinj.
+      + simpl in IH. apply IH. apply Hinj.
+      + apply eq_nat_dec.
+  Qed.
+
+  Lemma add_pc_safe_step : forall {n} (inp : input n) (pc : fin (S n)) i is acc st',
+    step_noswap inp (pc, is, acc) st' ->
+    exists st'', step_noswap inp (pc, (set_add Fin.eq_dec i is), acc) st''.
+  Proof.
+    intros n inp pc' i is acc st' Hstep.
+    inversion Hstep.
+    - eexists. apply step_noswap_add. apply H4.
+      apply set_mem_correct2. apply set_add_intro1.
+      apply set_mem_correct1 with Fin.eq_dec. assumption.
+    - eexists. eapply step_noswap_nop. apply H4.
+      apply set_mem_correct2. apply set_add_intro1.
+      apply set_mem_correct1 with Fin.eq_dec. assumption.
+    - eexists. eapply step_noswap_jmp. apply H3.
+      apply set_mem_correct2. apply set_add_intro1.
+      apply set_mem_correct1 with Fin.eq_dec. assumption.
+      apply H6.
+  Qed.
+
+  Lemma remove_pc_safe_run : forall {n} (inp : input n) i pc v acc st',
+    run_noswap inp (pc, set_add Fin.eq_dec i v, acc) st' ->
+    exists st'', run_noswap inp (pc, v, acc) st''.
+  Proof.
+    intros n inp i pc v acc st' Hr.
+    dependent induction Hr.
+    - eexists. eapply run_noswap_ok.
+    - eexists. eapply run_noswap_fail.
+      apply set_mem_complete1 in H.
+      apply set_mem_complete2.
+      intros Hin. apply H. apply set_add_intro. right. apply Hin.
+    - inversion H; subst; destruct (set_mem Fin.eq_dec pc' v) eqn:Hm.
+  Admitted.
+
+  Lemma add_pc_safe_run : forall {n} (inp : input n) i pc v acc st',
+    run_noswap inp (pc, v, acc) st' ->
+    exists st'', run_noswap inp (pc, (set_add Fin.eq_dec i v), acc) st''.
+  Proof.
+    intros n inp i pc v acc st' Hr.
+    destruct (set_mem Fin.eq_dec i v) eqn:Hm.
+    (* If i is already in the set, nothing changes. *)
+    rewrite set_add_idempotent.
+    exists st'. assumption. assumption.
+    (* Otherwise, the behavior might have changed.. *)
+    destruct (fin_big_or_small pc).
+    - (* If we're done, we're done no matter what. *)
+      eexists. rewrite H. eapply run_noswap_ok.
+    - (* The PC points somewhere inside. We tried (and maybe failed)
+         to execute and instruction. The challenging part
+         is that adding i may change the outcome from 'fail' to 'ok' *)
+      destruct H as [pc' Heq].
+      generalize dependent st'.
+      induction v using (@set_induction (fin n) Fin.eq_dec);
+      intros st' Hr.
+      + (* Our set of valid states is nearly empty. One step,
+           and it runs dry. *)
+        simpl. destruct (Fin.eq_dec pc' i) eqn:Heq_dec.
+        * (* The PC is the one allowed state. *)
+          remember (nth inp pc') as h. destruct h. destruct o.
+          { (* Addition. *)
+            destruct (fin_big_or_small (FS pc')).
+            - (* The additional step puts as at the end. *)
+              eexists. eapply run_noswap_trans.
+              + rewrite Heq. apply step_noswap_add.
+                symmetry. apply Heqh. simpl. rewrite Heq_dec. reflexivity.
+              + rewrite H. apply run_noswap_ok.
+            - (* The additional step puts us somewhere else. *)
+              destruct H as [f' H].
+              eexists. eapply run_noswap_trans.
+              + rewrite Heq. apply step_noswap_add.
+                symmetry. apply Heqh. simpl. rewrite Heq_dec. reflexivity.
+              + rewrite H. apply run_noswap_fail.
+                simpl. rewrite Heq_dec. reflexivity. }
+          { (* No-op *) admit. }
+          { (* Jump*) admit. }
+        * (* The PC is not. We're done. *)
+          eexists. rewrite Heq. eapply run_noswap_fail.
+          simpl. rewrite Heq_dec. reflexivity. 
+      + destruct (set_mem Fin.eq_dec a v) eqn:Hm'.
+        * unfold fin. rewrite (set_add_idempotent Fin.eq_dec a).
+
+            
+          { apply step_noswap_nop.
+            - symmetry. apply Heqh.
+            - simpl. rewrite Heq_dec. reflexivity. }
+
+      (*
+      dependent induction Hr; subst.
+      + (* We can't be in the OK state, since we already covered
+           that earlier. *)
+        destruct n. inversion pc'.
+        apply weaken_neq_to_fin in Heq as [].
+      + apply weaken_one_inj in Heq as Hs. subst.
+        destruct (Fin.eq_dec pc'0 i) eqn:Heq_dec.
+        * admit.
+        * eexists. eapply run_noswap_fail.
+          assert (~set_In pc'0 v).
+          { apply (set_mem_complete1 Fin.eq_dec). assumption. }
+          assert (~set_In pc'0 (List.cons i List.nil)).
+          { simpl. intros [Heq'|[]]. apply n0. auto. }
+          assert (~set_In pc'0 (set_union Fin.eq_dec v (List.cons i List.nil))).
+          { intros Hin. apply set_union_iff in Hin as [Hf|Hf].
+            - apply H0. apply Hf.
+            - apply H1. apply Hf. }
+          simpl in H2. apply set_mem_complete2. assumption.
+      + apply (add_pc_safe_step _ _ i) in H as [st''' Hr'].
+        eexists. eapply run_noswap_trans.
+        apply Hr'. destruct st' as [[pc'' v''] acc''].
+         specialize (IHHr i pc'' v'' acc'').*)
+
+
+    (*    intros n inp i pc v.
+    generalize dependent i.
+    generalize dependent pc.
+    induction v; intros pc i acc st Hr.
+    - inversion Hr; subst.
+      + eexists. apply run_noswap_ok.
+      + destruct (Fin.eq_dec pc' i) eqn:Heq_dec.
+        * admit.
+        * eexists. apply run_noswap_fail.
+          simpl. rewrite Heq_dec. reflexivity.
+      + inversion H; subst; simpl in H7; inversion H7.
+    - inversion Hr; subst.
+      + eexists. apply run_noswap_ok.
+      + destruct (Fin.eq_dec pc' i) eqn:Heq_dec.
+        * admit.
+        * eexists. apply run_noswap_fail.
+          simpl. rewrite Heq_dec. simpl in H4.
+          apply H4.
+      + 
+       destruct (nth inp pc') as [op t]. *)
+
+  Admitted.
+   
   Theorem valid_input_terminates  : forall n (inp : input n) st,
     valid_input inp -> exists st', run_noswap inp st st'.
   Proof.
+    intros n inp st.
+    destruct st as [[pc is] acc].
+    generalize dependent inp.
+    generalize dependent pc.
+    generalize dependent acc.
+    induction is using (@set_induction (fin n) Fin.eq_dec); intros acc pc inp Hv;
+    (* The PC may point past the end of the
+       array, or it may not. *)
+    destruct (fin_big_or_small pc);
+    (* No matter what, if it's past the end
+       of the array, we're done, *)
+    try (eexists (pc, _, acc); rewrite H; apply run_noswap_ok).
+    - (* It's not past the end of the array,
+         and the 'allowed' list is empty.
+         Evaluation fails. *)
+      destruct H as [f' Heq].
+      exists (pc, Datatypes.nil, acc).
+      rewrite Heq. apply run_noswap_fail. reflexivity.
+    - (* We're not past the end of the array. However,
+         adding a new valid index still guarantees
+         evaluation terminates. *)
+      specialize (IHis acc pc inp Hv) as [st' Hr].
+      apply add_pc_safe_run with st'. assumption.
+  Qed.
+
+  (*
+      (* It's not past the end of the array,
+         and we're in the inductive case on is. *)
+      destruct H as [pc' Heq].
+      destruct (Fin.eq_dec pc' a) eqn:Heq_dec.
+      + (* This PC is allowed. *)
+        (* That must mean we have a non-empty list. *)
+        remember (nth inp pc') as h. destruct h as [op t].
+        (* Unfortunately, we can't do eexists at the top
+           level, since that will mean the final state
+           has to be the same for every op. *)
+        destruct op.
+        (* Addition. *)
+        { destruct (IHis (M.add acc t) (FS pc') inp Hv) as [st' Htrans].
+          eexists. eapply run_noswap_trans.
+          rewrite Heq. apply step_noswap_add.
+          - symmetry. apply Heqh.
+          - simpl. rewrite Heq_dec. reflexivity.
+          - simpl. rewrite Heq_dec. apply Htrans. }
+        (* No-ops *)
+        { destruct (IHis acc (FS pc') inp Hv) as [st' Htrans].
+          eexists. eapply run_noswap_trans.
+          rewrite Heq. apply step_noswap_nop with t.
+          - symmetry. apply Heqh.
+          - simpl. rewrite Heq_dec. reflexivity. 
+          - simpl. rewrite Heq_dec. apply Htrans. }
+        (* Jump. *) 
+        { (* A little more interesting. We need to know that the jump is valid. *)
+          assert (Hv' : valid_inst (jmp, t) pc').
+          { specialize (Hv pc'). rewrite <- Heqh in Hv. assumption. }
+          inversion Hv'.
+          (* Now, proceed as usual. *)
+          destruct (IHis acc f' inp Hv) as [st' Htrans].
+          eexists. eapply run_noswap_trans.
+          rewrite Heq. apply step_noswap_jmp with t.
+          - symmetry. apply Heqh.
+          - simpl. rewrite Heq_dec. reflexivity. 
+          - apply H0.
+          - simpl. rewrite Heq_dec. apply Htrans. }
+      + (* The top PC is not allowed. *)
+        specialize (IHis acc pc inp Hv) as [st' Hr].
+     apply add_pc_safe_run with st'. assumption. *)
+  Qed.
+
+
     (* Stoppped here. *)
   Admitted.
 End DayEight.
